Coq

coq_alt/Mon.v
@@ -1,6 +1,8 @@
 Set Implicit Arguments.
 Require Import Strings.String CSC.Util CSC.Sets CSC.Props Coq.Program.Equality.
 
+Require Import Paco.paco.
+
 (** * This file defines the various monitors from the paper. *)
 
 (** General structure of monitors. This time as module for namespacing. *)
@@ -29,6 +31,8 @@ Module Monitor (M : MonitorT) <: MonitorT.
     is_value := fun _ => True;
   }.
   Definition tracepref := @Util.tracepref Trace__Instance.
+  (** Monitor traces must not stutter, which makes sense, because monitors should operate on relevant information. *)
+  (** The empty event is not relevant, in case you wondered. *)
   Inductive cong : Props.tracepref -> tracepref -> Prop :=
   | cong_refl : cong nil nil
   | cong_stutter_L : forall (b : AbsEv)
@@ -41,7 +45,7 @@ Module Monitor (M : MonitorT) <: MonitorT.
                        (Bs : tracepref)
                        (As : Props.tracepref),
       cong_e (Some a) None ->
-      cong As Bs ->
+      cong (List.cons a As) Bs ->
       cong (List.cons a As) Bs
   | cong_trans : forall (b : AbsEv)
                    (a : Props.Event)
@@ -53,6 +57,31 @@ Module Monitor (M : MonitorT) <: MonitorT.
   .
   #[export]
   Hint Constructors cong : core.
+
+  CoInductive ccong : Props.tracepref -> tracepref -> Prop :=
+  | ccong_refl : ccong nil nil
+  | ccong_stutter_L : forall (b : AbsEv)
+                       (Bs : tracepref)
+                       (As : Props.tracepref),
+      cong_e None (Some b) ->
+      ccong As (List.cons b Bs) ->
+      ccong As (List.cons b Bs)
+  | ccong_stutter_R : forall (a : Props.Event)
+                       (Bs : tracepref)
+                       (As : Props.tracepref),
+      cong_e (Some a) None ->
+      ccong (List.cons a As) Bs ->
+      ccong (List.cons a As) Bs
+  | ccong_trans : forall (b : AbsEv)
+                   (a : Props.Event)
+                   (Bs : tracepref)
+                   (As : Props.tracepref),
+      cong_e (Some a) (Some b) ->
+      ccong As Bs ->
+      ccong (List.cons a As) (List.cons b Bs)
+  .
+  #[export]
+  Hint Constructors ccong : core.
 
   Definition sat (As : Props.tracepref) : Prop :=
     exists (Bs : tracepref) (T : State),
@@ -530,7 +559,7 @@ Proof.
              end) (zip (opt As__TMS) (opt As__SMS))) in H.
       destruct (zip(opt As__TMS) (opt As__SMS)); easy.
     + destruct H1 as [H1__a H1__b]; subst. clear H. dependent induction H0.
-      repeat constructor. repeat constructor. now inv H. now apply IHcong. now inv H. now apply IHcong.
+      repeat constructor 1. now apply IHcong.
   - destruct a as [a__TMS a__SMS];
     symmetry in H; apply zip_cons in H; deex; destruct H as [H'__a [H'__b H'__c]].
     apply opt_some in H'__a, H'__b; deex; destruct H'__a as [H'a1 [H'a2 H'a3]]; destruct H'__b as [H'b1 [H'b2 H'b3]].
@@ -593,18 +622,29 @@ Lemma MSMon_cong_cons_split (As : tracepref) (a__TMS : option TMSMon.AbsEv) (a__
   )
 .
 Proof.
-  intros H; dependent induction As; eauto.
-  - right; repeat split. inv H. inv H3. inv H. inv H0. constructor. inv H. inv H3. inv H. inv H0. constructor.
-    easy.
-Admitted.
+  revert a__TMS a__SMS As__MS; induction As; intros.
+  - inv H; inv H3; right; repeat split; trivial.
+  - dependent induction H; eauto.
+    inv H; left; exists a; exists As; now repeat split.
+Qed.
 Lemma MSMon_cong_none_strip (As : tracepref) Bs :
-  MSMon.cong As ((None, None) :: Bs)%list ->
-  MSMon.cong As Bs
+  MSMon.ccong As ((None, None) :: Bs)%list ->
+  MSMon.ccong As Bs
 .
 Proof.
-  intros H; dependent induction H; eauto.
-  - constructor; trivial. now eapply IHcong.
-  - inv H. inv H1; inv H2; now repeat constructor.
+  intros H. pcofix CH; intros H0. destruct H0.
+  -
+  - apply CH. assumption.
+  - constructor 3. assumption. now apply CH.
+  - constructor 3. inv H; constructor; assumption. apply CH. constructor 4. exact H. exact H0.
+Qed.
+  inv H0.
+  - inv H5. apply H. easy. constructor 3. easy. now apply H. constructor 3. inv H3; now constructor.
+    apply H. constructor 4. easy. assumption.
+  - inv H2. constructor 3. assumption. apply H; assumption.
+    constructor 3. assumption. now apply H.
+    apply H. constructor 4; assumption.
+  - constructor 3. inv H4. constructor; auto. apply H. constructor 4; auto.
 Qed.
 Lemma MSMon_steps_split_cong (T1 T1' : TMSMon.AbsState) (T2 T2' : SMSMon.AbsState) As Xs :
   MSMon.cong Xs As ->
